src/Analysis/Instances/Congruence/Congruence_Print.thy
@@ -1,0 +1,25 @@
+theory Congruence_Print
+  imports Congruence_Domain
+begin
+
+section \<open>Congruence printing\<close>
+
+subsection \<open>Printable instance\<close>
+
+definition string_of_congruence :: "congruence \<Rightarrow> string" where
+  "string_of_congruence c =
+     (case Rep_congruence c of
+        None \<Rightarrow> ''Top''
+      | Some (r, m) \<Rightarrow>
+          if m = 0 then ''='' @ show_int r
+          else ''='' @ show_int r @ '' (mod '' @ show_int m @ '')'')"
+
+instantiation congruence :: show_val begin
+definition "show_val_congruence (c :: congruence) = string_of_congruence c"
+instance ..
+end
+
+lemma show_val_congruence_eq [simp]: "(show_val :: congruence \<Rightarrow> string) = string_of_congruence"
+  unfolding show_val_congruence_def by simp
+
+end
